@prefix : <#> .
@prefix rdf: <http://www.w3.org/1999/02/22-rdf-syntax-ns#> .
@prefix xsd: <http://www.w3.org/2001/XMLSchema#> .
@prefix rdfs: <http://www.w3.org/2000/01/rdf-schema#> .
@prefix dcterms: <http://purl.org/dc/terms/> .


<>
  dcterms:issued "2020-07-01"^^xsd:date ;
  dcterms:modified "2020-07-01"^^xsd:date ;
  rdfs:label "ShapeTree terms"@en .


# ShapeTree Class
#############################################################################
# Defines a tree of related resources which combine to enable some task
# see: https://shapetrees.github.io/specification/primer
#############################################################################
:ShapeTree 
  a rdfs:Class ;
  rdfs:comment "Defines a tree of related resources which combine to enable some task"@en ;
  rdfs:isDefinedBy <> ;
  rdfs:label "ShapeTree"@en .

# Properties in domain of ShapeTree
#########################################################
:expectsType 
  a rdf:Property ;
  rdfs:domain :ShapeTree ;
  rdfs:range :ShapeTreeExpectedResourceType ;
  rdfs:comment "Describes the expected type of resource the ShapeTree will create."@en ;
  rdfs:isDefinedBy <> ;
  rdfs:label "Expects Type"@en .

:hasContents 
  a rdf:Property ;
  rdfs:domain :ShapeTree ;
  rdfs:range :ShapeTree ;
  rdfs:comment "Links a ShapeTree to another ShapeTree that is directly contained within its planted container"@en ;
  rdfs:isDefinedBy <> ;
  rdfs:label "Has Contents"@en .

:hasReferences 
  a rdf:Property ;
  rdfs:domain :ShapeTree ;
  rdfs:range :ShapeTreeReference ;
  rdfs:isDefinedBy <> ;
  rdfs:comment "Links a ShapeTree to a ShapeTreeReference"@en ;
  rdfs:label "Has References"@en .

:nameTemplatedBy 
  a rdf:Property ;
  rdfs:domain :ShapeTree ;
  rdfs:comment "Describes a URI Template (RFC 6570) that governs the naming of resources of this ShapeTree"@en ;
  rdfs:isDefinedBy <> ;
  rdfs:label "Name Templated By"@en .

:validatedBy 
  a rdf:Property ;
  rdfs:domain :ShapeTree ;
  rdfs:comment "Links a ShapeTree to a Shape"@en ;
  rdfs:isDefinedBy <> ;
  rdfs:label "Validated By"@en .

# Properties in the range of ShapeTree
#############################################################################
# usesTree is a generalized property for when a a reference 
# to a ShapeTree is required
#############################################################################
:usesTree 
  a rdf:Property ;
  rdfs:domain :ShapeTreeLabel ;
  rdfs:range :ShapeTree ;
  rdfs:comment "Links to a ShapeTree"@en ;
  rdfs:isDefinedBy <> ;
  rdfs:label "Uses ShapeTree"@en .



# ShapeTreeExpectedResourceType Class
#############################################################################
# Defines an enumeration of generalized resource types that describe the
# type of resource the planted ShapeTree is expected to validate against
# Implementations of ShapeTree will map these generalized values to
# specific implemtnations (LDP, etc.)
#############################################################################
:ShapeTreeExpectedResourceType 
  a rdfs:Class ;
  rdfs:comment "Defines an enumerable set of resource types expected by a given ShapeTree"@en ;
  rdfs:isDefinedBy <> ;
  rdfs:label "ShapeTreeExpectedResourceType"@en .


# ShapeTreeContainer class
#############################################################################
# A sub-class of ShapeTreeExpectedResourceType this class represents
# a generalized container
#############################################################################
:ShapeTreeContainer 
  a rdfs:Class ;
  rdfs:subClassOf :ShapeTreeExpectedResourceType ;
  rdfs:comment "Describes a generalized container within a ShapeTree ecosystem"@en ;
  rdfs:isDefinedBy <> ;
  rdfs:label "ShapeTreeContainer"@en .


# ShapeTreeResource class
#############################################################################
# A sub-class of ShapeTreeExpectedResourceType this class represents
# a generalized resource
#############################################################################
:ShapeTreeResource 
  a rdfs:Class ;
  rdfs:subClassOf :ShapeTreeExpectedResourceType ;
  rdfs:comment "Describes a generalized resource (non-container) within a ShapeTree ecosystem"@en ;
  rdfs:isDefinedBy <> ;
  rdfs:label "ShapeTreeResource"@en .


# ShapeTreeReference class
#############################################################################
# A ShapeTreeReference provides the necessary context to associate instance
# data between related ShapeTrees via a ShapePath
#############################################################################
:ShapeTreeReference 
  a rdfs:Class ;
  rdfs:comment "Describes how a ShapeTree references another ShapeTree via a ShapePath"@en ;
  rdfs:isDefinedBy <> ;
  rdfs:label "ShapeTreeReference"@en .

# Properties in domain of ShapeTreeReference
#########################################################
:traversedViaShapePath
  a rdf:Property ;
  rdfs:domain :ShapeTreeReference ;
  rdfs:comment "Describes how one ShapeTree traverses its instance data to reach another ShapeTree"@en ;
  rdfs:isDefinedBy <> ;
  rdfs:label "Traversed Via ShapePath"@en .


# UiStringsIndex class
#############################################################################
# A UiStringsIndex details a ShapeTree in a human-readable way.
# It is primarily used for use cases where a ShapeTree must be described to
# a user for purposes of authorization.
#############################################################################
:UiStringsIndex 
  a rdfs:Class ;
  rdfs:comment "Provides an index of SKOS poly-hierarchies which can be used to describe a ShapeTree"@en ;
  rdfs:isDefinedBy <> ;
  rdfs:label "UiStringsIndex"@en .

# Properties in domain of UiStringsIndex
#########################################################
:hasSeries
  a rdf:Property ;
  rdfs:domain :UiStringsIndex ;
  rdfs:range :UiStringsSeries ;
  rdfs:comment "Links between a UiStringsIndex and a UiStringsSeries"@en ;
  rdfs:isDefinedBy <> ;
  rdfs:label "Has Series"@en .

# UiStringsSeries class
#############################################################################
# A UiStringsSeries details a versioned set of UiStringsHierarchy classes
# Primary use is grouping UiStringsHierarchy instances by a common discriminator
# such as language or intended audience
#############################################################################
:UiStringsSeries 
  a rdfs:Class ;
  rdfs:comment "Groups a set of UiStringsHierarchy by a given discriminator"@en ;
  rdfs:isDefinedBy <> ;
  rdfs:label "UiStringsSeries"@en .

# Properties in domain of UiStringsSeries
#########################################################
:hasStringsHierarchy
  a rdf:Property ;
  rdfs:domain :UiStringsSeries ;
  rdfs:range :UiStringsHierarchy ;
  rdfs:comment "Links between a UiStringsSeries and a UiStringsHierarchy"@en ;
  rdfs:isDefinedBy <> ;
  rdfs:label "Has Strings Hierarchy"@en .

# UiStringsHierarchy class
#############################################################################
# A UiStringsHierarchy details a versioned SKOS poly-hierarchy that describes
# a ShapeTree in a given language or format for an intended audience 
# (decreased cognitivty ability, etc.)
#############################################################################
:UiStringsHierarchy 
  a rdfs:Class ;
  rdfs:comment "Describes a SKOS poly-hierarchy for purproses of labeling a ShapeTree"@en ;
  rdfs:isDefinedBy <> ;
  rdfs:label "UiStringsHierarchy"@en .

# Properties in domain of UiStringsHierarchy
#########################################################
:hasVersion
  a rdf:Property ;
  rdfs:domain :UiStringsHierarchy ;
  rdfs:comment "Describes the version of a UiStringsSeries"@en ;
  rdfs:isDefinedBy <> ;
  rdfs:label "Has Version"@en .

:hasSHA3256Hash
  a rdf:Property ;
  rdfs:domain :UiStringsHierarchy ;
  rdfs:comment "Describes the SHA3-256 of a UiStringsSeries"@en ;
  rdfs:isDefinedBy <> ;
  rdfs:label "Has SHA3-256 Hash"@en .

:hasSkosGraph
  a rdf:Property ;
  rdfs:domain :UiStringsHierarchy ;
  rdfs:range :ShapeTreeLabel ;
  rdfs:comment "Represents the IRI to the SKOS graph described by UiStringsHierarchy instance"@en ;
  rdfs:isDefinedBy <> ;
  rdfs:label "Has SKOS Graph"@en .

# ShapeTreeLabel class
#############################################################################
# A ShapeTreeLabel details the association between a label within a SKOS graph
# (detailed by UiStringsHierarchy) and a ShapeTree
#############################################################################
:ShapeTreeLabel 
  a rdfs:Class ;
  rdfs:comment "Describes the association between a SKOS label and a ShapeTree"@en ;
  rdfs:isDefinedBy <> ;
  rdfs:label "ShapeTreeLabel"@en .

